feat: finish formal exercises in ImpCEvalFun

ImpCEvalFun.v
@@ -199,7 +199,7 @@ Example example_test_ceval :
         end }>
 
      = Some (2, 0, 4).
-Proof. reflexivity. Qed.
+Proof. cbv. reflexivity. Qed.
 
 (** **** Exercise: 2 stars, standard, especially useful (pup_to_n)
 
@@ -207,16 +207,18 @@ Proof. reflexivity. Qed.
    [X] (inclusive: [1 + 2 + ... + X]) in the variable [Y].  Make sure
    your solution satisfies the test that follows. *)
 
-Definition pup_to_n : com
-  (* REPLACE THIS LINE WITH ":= _your_definition_ ." *). Admitted.
+Definition pup_to_n : com := <{
+  Y := 0;
+  while (X > 0) do
+    Y := Y + X;
+    X := X - 1
+  end
+}>.
 
 Example pup_to_n_1 :
   test_ceval (X !-> 5) pup_to_n
   = Some (0, 15, 0).
-(* FILL IN HERE *) Admitted.
-(* 
-Proof. reflexivity. Qed.
-*)
+Proof. cbv. reflexivity. Qed.
 (** [] *)
 
 (** **** Exercise: 2 stars, standard, optional (peven)
@@ -225,9 +227,20 @@ Proof. reflexivity. Qed.
     sets [Z] to [1] otherwise.  Use [test_ceval] to test your
     program. *)
 
-(* FILL IN HERE
+Definition peven : com := <{
+  while X > 1 do
+    X := X - 2
+  end;
+  Z := X
+}>.
 
-    [] *)
+Example peven_1 :
+  test_ceval (X !-> 8) peven = Some (0, 0, 0).
+Proof. cbv. reflexivity. Qed.
+
+Example peven_2 :
+  test_ceval (X !-> 7) peven = Some (1, 0, 1).
+Proof. cbv. reflexivity. Qed.
 
 (* ################################################################# *)
 (** * Relational vs. Step-Indexed Evaluation *)
@@ -360,7 +373,36 @@ Theorem ceval__ceval_step: forall c st st',
 Proof.
   intros c st st' Hce.
   induction Hce.
-  (* FILL IN HERE *) Admitted.
+  - exists 1. simpl. reflexivity.
+  - exists 1. simpl. rewrite H. reflexivity.
+  - destruct IHHce1 as [i1 IH1]. destruct IHHce2 as [i2 IH2].
+    exists (i1 + i2). destruct i1. discriminate IH1.
+    destruct i2. discriminate IH2. simpl.
+    assert (H: ceval_step st c1 (i1 + S i2) = Some st'). {
+      apply ceval_step_more with (i1 := S i1).
+      - rewrite <- plus_n_Sm. apply le_n_S. apply le_add_r.
+      - apply IH1.
+    }
+    rewrite H. apply ceval_step_more with (i1 := S i2).
+    + rewrite <- plus_n_Sm. apply le_n_S. apply le_add_l.
+    + apply IH2. 
+  - destruct IHHce as [i IH]. exists (S i). simpl.
+    rewrite H. apply IH.
+  - destruct IHHce as [i IH]. exists (S i). simpl.
+    rewrite H. apply IH.
+  - exists 1. simpl. rewrite H. reflexivity.
+  - destruct IHHce1 as [i1 IH1]. destruct IHHce2 as [i2 IH2].
+    exists (i1 + i2). destruct i1. discriminate IH1.
+    destruct i2. discriminate IH2. simpl. rewrite H.
+    assert (H': ceval_step st c (i1 + S i2) = Some st'). {
+      apply ceval_step_more with (i1 := S i1).
+      - rewrite <- plus_n_Sm. apply le_n_S. apply le_add_r.
+      - apply IH1.
+    }
+    rewrite H'. apply ceval_step_more with (i1 := S i2).
+    + rewrite <- plus_n_Sm. apply le_n_S. apply le_add_l.
+    + apply IH2.
+Qed. 
 (** [] *)
 
 Theorem ceval_and_ceval_step_coincide: forall c st st',
